examples/rv2/ISA.v
@@ -1,6 +1,6 @@
 Inductive memory_model  := RVWMO.
 Inductive base_standard := RV32I | RV64I.
-Inductive extension     := RVM   | RVA | RVF | RVD | RVQ | RVZiCSR | RVZifencei.
+Inductive extension     := RVM | RVA | RVF | RVD | RVQ | RVZiCSR | RVZifencei.
 
 Record ISA := {
   ISA_memory_model  : memory_model;
